rt ainvs: proved perform_invocation_valid_sched
This proof required two significant subproofs:
-- invoke_sched_context_valid_sched
-- invoke_sched_control_configure_valid_sched

Also in this commit:
 - Added commit_time_valid_sched (sorried)
 - Resolved a trivial sorry in ArchKernelInit_AI.thy
 - updates proofs that broke when sched_context_yield_to, handle_yield,
and sched_context_control_configure were updated in aspec.

proof/invariant-abstract/Invariants_AI.thy
@@ -269,6 +269,7 @@ abbreviation "sc_ntfn_sc_at \<equiv> sc_at_pred sc_ntfn"
 abbreviation "sc_tcb_sc_at \<equiv> sc_at_pred sc_tcb"
 abbreviation "sc_yf_sc_at \<equiv> sc_at_pred sc_yield_from"
 abbreviation "sc_replies_sc_at \<equiv> sc_at_pred sc_replies"
+abbreviation "sc_refills_sc_at \<equiv> sc_at_pred sc_refills"
 
 lemma sc_at_pred_def:
   "sc_at_pred proj P \<equiv> obj_at (\<lambda>ko. \<exists>sc n. ko = SchedContext sc n \<and> P (proj sc))"
@@ -278,6 +279,7 @@ lemmas sc_ntfn_sc_at_def = sc_at_pred_def[of sc_ntfn]
 lemmas sc_tcb_sc_at_def = sc_at_pred_def[of sc_tcb]
 lemmas sc_yf_sc_at_def = sc_at_pred_def[of sc_yield_from]
 lemmas sc_replies_sc_at_def = sc_at_pred_def[of sc_replies]
+lemmas sc_refills_sc_at_def = sc_at_pred_def[of sc_refills]
 
 lemma sc_at_pred_ko_atI:
   "ko_at (SchedContext sc nb) ptr s \<Longrightarrow> P (proj sc)
